src/core/DY.Core.Trace.State.Properties.fst
@@ -2,21 +2,262 @@ module DY.Core.Trace.State.Properties
 
 open FStar.List.Tot
 
+open DY.Core.List
 open DY.Core.Bytes.Type
 open DY.Core.Bytes
 open DY.Core.Label.Type
 open DY.Core.Trace.Type
 open DY.Core.Trace.PrefixSuffix
 open DY.Core.Trace.State.Aux
+open DY.Core.Trace.State.NoSetStateEntry
 open DY.Core.Trace.Manipulation
 open DY.Core.List
 
 module List = FStar.List.Tot.Base
+module ListProps = FStar.List.Tot.Properties
 
 
 
-let no_set_state_entry_for_p (p:principal) (tr:trace) =
-  forall sid. no_set_state_entry_for p sid tr
+open DY.Core.Trace.Invariant
+
+/// the session predicate remains true
+/// if the trace grows
+/// but there are no more state entries for the principal and the session
+
+val session_pred_later_:
+  {|cinvs: crypto_invariants |} -> {|sp:state_predicate cinvs |} ->
+  tr1:trace -> tr2:trace  -> p:principal -> sid:state_id -> cont:state_raw ->
+  Lemma
+    (requires 
+        tr1 <$ tr2 
+      /\ no_set_state_entry_for p sid (tr2 `suffix_after` tr1)
+      /\ sp.session_pred tr1 (get_session_aux p sid tr1) p sid cont
+    )
+    (ensures sp.session_pred tr2 (get_session_aux p sid tr2) p sid cont)
+let session_pred_later_ #_ #sp tr1 tr2 p sid cont =
+  get_session_aux_same p sid tr1 tr2;
+  let session = get_session_aux p sid tr1 in
+  sp.session_pred_grows tr1 tr2 session p sid cont
+
+let session_pred_later {|invs:protocol_invariants|} = session_pred_later_ #invs.crypto_invs #invs.trace_invs.state_pred
+
+
+
+
+
+(*** Properties of get_state ***)
+
+
+val get_state_state_was_set :
+  p:principal -> sid:state_id -> tr:trace ->
+  Lemma
+    (requires True)
+    (ensures (
+       let (opt_content, tr_out) = get_state p sid tr in
+       tr == tr_out /\
+       (match opt_content with
+       | None -> True
+       | Some v -> state_was_set tr p sid v
+       )
+      )
+    )
+    [SMTPat (get_state p sid tr)]
+let  get_state_state_was_set p sid tr =
+  normalize_term_spec get_state
+
+
+let rec get_state_no_set_state_for_on_suffix_after_event
+  (tr:trace) (p:principal) (sid:state_id) :
+  Lemma 
+  (requires Some? (fst (get_state p sid tr))
+  )
+  ( ensures (
+    let (Some st , _) = get_state p sid tr in
+    no_set_state_entry_for p sid (tr `suffix_after_event` (SetState p sid st)) 
+    )
+  )
+= let (Some st , _) = get_state p sid tr in
+  reveal_opaque (`%get_state) get_state; 
+  match tr with
+  | Nil -> ()
+  | Snoc init (SetState p' sid' cont') -> 
+         if p' = p && sid' = sid
+           then ()
+           else ( 
+             get_state_no_set_state_for_on_suffix_after_event init p sid;
+             suffix_after_event_init tr (SetState p' sid' cont')
+           )
+  | Snoc init ev -> 
+    get_state_no_set_state_for_on_suffix_after_event init p sid;
+    suffix_after_event_init tr (SetState p sid st)
+
+(*** Properties of get_session ***)
+
+let rec get_session_grows (p:principal) (sid:state_id) (tr1 tr2:trace):
+  Lemma
+  ( requires tr1 <$ tr2 /\ Some? (get_session p sid tr1)
+  )
+  (ensures
+    Some? (get_session p sid tr2)
+  )
+ = reveal_opaque (`%grows) grows; 
+   norm_spec [zeta; delta_only [`%prefix]] (prefix);
+   if tr1 = tr2 
+   then ()
+   else (
+     match tr2 with
+     | Nil -> ()
+     | Snoc init _ -> get_session_grows p sid tr1 init
+   )
+
+
+
+let rec get_session_state_was_set (p:principal) (sid:state_id) (tr:trace):
+  Lemma
+  (requires Some? (get_session p sid tr))
+  (ensures exists cont. state_was_set tr p sid cont )
+  = match tr with
+  | Nil -> ()
+  | Snoc init (SetState p' sid' cont') -> (
+         if p' = p && sid' = sid
+         then ()
+         else get_session_state_was_set p sid init
+   )      
+  | Snoc init _ -> 
+        get_session_state_was_set p sid init
+
+
+
+(*** Relations of get_state and get_session ***)
+
+
+
+val get_state_aux_is_last_of_get_session_aux:
+  p:principal -> sid:state_id -> tr:trace ->
+  Lemma 
+    (requires True
+    )
+    (ensures (
+      let session = get_session_aux p sid tr in
+      match get_state_aux p sid tr with
+      | None -> Nil? session
+      | Some st -> Snoc? session /\ (let Snoc _ last = session in st = last)
+    )
+    )
+let rec get_state_aux_is_last_of_get_session_aux p sid tr = 
+  match tr with
+  | Nil -> ()
+  | Snoc init _ -> get_state_aux_is_last_of_get_session_aux p sid init
+
+
+/// relating get_state and get_session
+
+val get_state_is_last_of_get_session:
+  p:principal -> sid:state_id -> tr:trace ->
+  Lemma 
+    (requires True
+    )
+    (ensures (
+      let opt_session = get_session p sid tr in
+      let (opt_state, _) = get_state p sid tr in
+      match opt_state with
+      | None -> None? opt_session
+      | Some st -> 
+          Some? opt_session /\ Snoc? (Some?.v opt_session) /\ (let Some (Snoc _ last) = opt_session in st = last)
+    )
+    )
+    [SMTPat (get_session p sid tr); SMTPat (get_state p sid tr)]
+let get_state_is_last_of_get_session p sid tr =
+    reveal_opaque (`%get_state) (get_state);
+    get_state_aux_is_last_of_get_session_aux p sid tr
+
+
+
+(*** Relation of get_state, get_session and get_full_state ***)
+
+
+/// The main relation:
+/// if the principal has a full state on the trace
+/// and the state id appears in the full state,
+/// then
+/// the entry in full state related to state id is exactly the session
+/// and
+/// the last entry of the session is get state
+
+let full_state_some_get_session_get_state (p:principal) (sid:state_id) (tr:trace):
+  Lemma 
+  (requires
+       Some? (get_full_state p tr)
+     /\ sid `List.mem` (List.map fst (Some?.v (get_full_state p tr)))
+  )
+  (ensures (
+     let Some full_st = get_full_state p tr in
+     let session_opt = get_session p sid tr in
+     let (state_opt, _) = get_state p sid tr in
+
+     Some? session_opt
+     /\ (let Some sess = session_opt in
+        ((sid, sess) `List.mem` full_st)
+        /\ ( Snoc? sess 
+          /\ (let Snoc _ last = sess in
+             Some? state_opt /\ Some?.v state_opt = last
+            )
+          )
+       )
+   )
+  )
+  = let Some full_st = get_full_state p tr in
+    FStar.List.Tot.Properties.memP_map_elim fst sid full_st;
+    eliminate exists sess. (sid, sess) `List.mem` full_st 
+    returns Some? (get_session p sid tr) /\ ( (sid, Some?.v (get_session p sid tr)) `List.mem` full_st )
+    with _ . (
+      mem_choose_elim 
+        (get_session_indexed tr p) 
+        (zero_to_sid (compute_new_session_id p tr)) 
+        (sid, sess)
+        )
+
+
+
+// corolloray of the above:
+// the entries (si, c) in full state satisfy:
+// c = get_session si
+let full_state_mem_get_session (tr:trace) (p:principal) :
+  Lemma
+  (requires Some? (get_full_state p tr))
+  (ensures (
+    let Some full_st = get_full_state p tr in
+    forall si c. (si, c) `List.mem` full_st  ==> Some c = get_session p si tr
+  ))
+  =     
+  let Some full_st = get_full_state p tr in
+  introduce forall si c. (si, c) `List.mem` full_st ==> Some c = get_session p si tr
+  with(
+    introduce _ ==> _
+    with _ . (
+ mem_choose_elim (get_session_indexed tr p) (zero_to_sid (compute_new_session_id p tr)) (si,c);
+  full_state_some_get_session_get_state p si tr
+    )
+  )
+
+(*** Properties of compute_new_session_id ***)
+
+
+val compute_new_session_id_larger_than_id_on_trace:
+  prin:principal -> tr:trace ->
+  sess_id:state_id -> state_content:bytes ->
+  Lemma
+  (requires event_exists tr (SetState prin sess_id state_content))
+  (ensures sess_id.the_id < (compute_new_session_id prin tr).the_id)
+let rec compute_new_session_id_larger_than_id_on_trace prin tr sess_id state_content =
+  match tr with
+  | Nil -> ()
+  | Snoc tr_init evt -> (
+    if evt = SetState prin sess_id state_content then ()
+    else (
+      compute_new_session_id_larger_than_id_on_trace prin tr_init sess_id state_content
+    )
+  )
 
 let rec compute_new_session_id_same (p:principal) (tr1 tr2:trace) :
   Lemma (
@@ -82,27 +323,6 @@ let rec zero_to_sid_mems (bound:state_id) (sid:state_id) :
      )
   )
 
-
-let get_full_state_same (p:principal) (tr1:trace) (tr2:trace):
-  Lemma
-  (requires
-      tr1 <$ tr2 /\ 
-      no_set_state_entry_for_p p (tr2 `suffix_after` tr1)
-    )
-  (ensures get_full_state p tr1 = get_full_state p tr2)
-= introduce forall sid. get_session_indexed tr1 p sid = get_session_indexed tr2 p sid
-  with (
-    reveal_opaque (`%get_session) get_session; 
-    get_session_aux_same p sid tr1 tr2
-  ); 
-  compute_new_session_id_same p tr1 tr2;
-  choose_equals
-    (get_session_indexed tr1 p) 
-    (get_session_indexed tr2 p) 
-    (zero_to_sid (compute_new_session_id p tr1))
-  
-
-
 let rec compute_new_session_id_grows (p:principal) (tr1 tr2:trace):
   Lemma 
   (requires tr1 <$ tr2
@@ -122,78 +342,7 @@ let rec compute_new_session_id_grows (p:principal) (tr1 tr2:trace):
 
 
 
-val full_state_session_lemma:
-  (tr:trace) -> (p:principal) -> (sid:state_id) -> (sess:_) ->
-  Lemma
-  (requires
-        Some? (get_full_state p tr)
-      /\ (sid, sess) `List.mem` (Some?.v (get_full_state p tr))
-  )
-  ( ensures (
-    let Some full_st = get_full_state p tr in
-    get_session p sid tr = Some sess
-      )
-  )
-let full_state_session_lemma tr p sid sess =
-  mem_choose_elim 
-    (get_session_indexed tr p) 
-    (zero_to_sid (compute_new_session_id p tr)) 
-    (sid, sess)
-
-let full_state_some_get_session_some (p:principal) (sid:state_id) (tr:trace):
-  Lemma 
-  (requires
-     Some? (get_full_state p tr)
-     /\ sid `List.mem` (List.map fst (Some?.v (get_full_state p tr)))
-  )
-  (ensures
-     Some? (get_session p sid tr)
-  )
-  = let Some full_st = get_full_state p tr in
-    let next_sid = compute_new_session_id p tr in
-    let sids = zero_to_sid next_sid in
-    FStar.List.Tot.Properties.memP_map_elim fst sid full_st;
-    eliminate exists sess. (sid, sess) `List.mem` full_st 
-    returns Some? (get_session p sid tr)
-    with _ .
-      mem_choose_elim (get_session_indexed tr p) sids (sid, sess)
-    
-
-
-let rec get_session_grows (p:principal) (sid:state_id) (tr1 tr2:trace):
-  Lemma
-  ( requires tr1 <$ tr2 /\ Some? (get_session p sid tr1)
-  )
-  (ensures
-    Some? (get_session p sid tr2)
-  )
- = reveal_opaque (`%grows) grows; 
-   norm_spec [zeta; delta_only [`%prefix]] (prefix);
-   if tr1 = tr2 
-   then ()
-   else (
-     match tr2 with
-     | Nil -> ()
-     | Snoc init _ -> get_session_grows p sid tr1 init
-   )
-
-
-
-let rec get_session_state_was_set (p:principal) (sid:state_id) (tr:trace):
-  Lemma
-  (requires Some? (get_session p sid tr))
-  (ensures exists cont. state_was_set tr p sid cont )
-  = match tr with
-  | Nil -> ()
-  | Snoc init (SetState p' sid' cont') -> (
-         if p' = p && sid' = sid
-         then ()
-         else get_session_state_was_set p sid init
-   )      
-  | Snoc init _ -> 
-        get_session_state_was_set p sid init
-
-
+(*** More Relation on get_session and get_full_state ***)
 
 let get_session_some_full_state_some (p:principal) (sid:state_id) (tr:trace):
   Lemma 
@@ -209,6 +358,27 @@ let get_session_some_full_state_some (p:principal) (sid:state_id) (tr:trace):
         compute_new_session_id_larger_than_id_on_trace p tr sid cont
 
 
+(*** Properties of get_full_state ***)
+
+let get_full_state_same (p:principal) (tr1:trace) (tr2:trace):
+  Lemma
+  (requires
+      tr1 <$ tr2 /\ 
+      no_set_state_entry_for_p p (tr2 `suffix_after` tr1)
+    )
+  (ensures get_full_state p tr1 = get_full_state p tr2)
+= introduce forall sid. get_session_indexed tr1 p sid = get_session_indexed tr2 p sid
+  with (
+    reveal_opaque (`%get_session) get_session; 
+    get_session_aux_same p sid tr1 tr2
+  ); 
+  compute_new_session_id_same p tr1 tr2;
+  choose_equals
+    (get_session_indexed tr1 p) 
+    (get_session_indexed tr2 p) 
+    (zero_to_sid (compute_new_session_id p tr1))
+
+
 let full_state_fst_zero_to_sid (tr:trace) (p:principal):
   Lemma
   ( requires Some? (get_full_state p tr)
@@ -217,7 +387,7 @@ let full_state_fst_zero_to_sid (tr:trace) (p:principal):
     let Some full_st = get_full_state p tr in
     let next_sid = compute_new_session_id p tr in
     (List.map fst (full_st)) `List.subset` (zero_to_sid next_sid)
-    )
+   )
   )
   =
     let Some full_st = get_full_state p tr in
@@ -230,12 +400,10 @@ let full_state_fst_zero_to_sid (tr:trace) (p:principal):
       eliminate exists sess. (sid, sess) `List.mem` full_st
       returns _
       with _ . (
-      mem_choose_elim (get_session_indexed tr p) (zero_to_sid next_sid) (sid,sess)      
+      mem_choose_elim (get_session_indexed tr p) (zero_to_sid next_sid) (sid,sess)    
       )
     )
   )
-
-
 
 let get_full_state_on_growing_traces (p:principal) (tr1 tr2:trace) (sid:state_id):
   Lemma 
@@ -250,24 +418,25 @@ let get_full_state_on_growing_traces (p:principal) (tr1 tr2:trace) (sid:state_id
   )
   = 
   let Some full_st1 = get_full_state p tr1 in
- 
-         let new_sid1 = compute_new_session_id p tr1 in
-         let new_sid2 = compute_new_session_id p tr2 in
-         compute_new_session_id_grows p tr1 tr2;
-         let sids1 = zero_to_sid new_sid1 in
-         let sids2 = zero_to_sid new_sid2 in
-         full_state_fst_zero_to_sid tr1 p;
-           zero_to_sid_mems new_sid1 sid;
-           zero_to_sid_mem new_sid2 sid;
-         
-         full_state_some_get_session_some p sid tr1;
-         get_session_grows p sid tr1 tr2;
-         let Some sess2 = get_session p sid tr2 in
-         get_session_some_full_state_some p sid tr2;
-         let Some full_st2 = get_full_state p tr2 in
-         mem_choose (get_session_indexed tr2 p) sids2 sid;
-         FStar.List.Tot.Properties.memP_map_intro fst (sid, sess2) full_st2
+  let new_sid1 = compute_new_session_id p tr1 in
+  let new_sid2 = compute_new_session_id p tr2 in
+  compute_new_session_id_grows p tr1 tr2;
+  let sids1 = zero_to_sid new_sid1 in
+  let sids2 = zero_to_sid new_sid2 in
+  full_state_fst_zero_to_sid tr1 p;
+  zero_to_sid_mems new_sid1 sid;
+  zero_to_sid_mem new_sid2 sid;
+
+  full_state_some_get_session_get_state p sid tr1;
+  get_session_grows p sid tr1 tr2;
+  let Some sess2 = get_session p sid tr2 in
+  get_session_some_full_state_some p sid tr2;
+  let Some full_st2 = get_full_state p tr2 in
+  mem_choose (get_session_indexed tr2 p) sids2 sid;
+  FStar.List.Tot.Properties.memP_map_intro fst (sid, sess2) full_st2
    
+(*** More Relations on get_state and get_full_state ***)
+
 
 let rec state_was_set_full_state (tr:trace) (p:principal) (sid:state_id) (cont:bytes):
   Lemma
@@ -310,109 +479,40 @@ let rec state_was_set_full_state (tr:trace) (p:principal) (sid:state_id) (cont:b
      get_full_state_same p init tr;
      state_was_set_full_state init p sid cont
 
-val parse_full_state_lemma :
-  (tr: trace) -> p:principal -> (sid:state_id) -> (init: _) -> (last:_) ->
+val get_state_get_full_state:
+  tr:trace -> p:principal -> sid:state_id ->
   Lemma 
-  (requires
-       Some? (get_full_state p tr) 
-     /\ (sid, (Snoc init last)) `List.mem` (Some?.v (get_full_state p tr))
+  ( requires Some? (fst (get_state p sid tr))
   )
-    ( ensures (
-      let Some full_st = get_full_state p tr in
-        Some?   (fst (get_state p sid tr))
-      /\ Some?.v (fst (get_state p sid tr)) = last
-      )
-
-    )
-let parse_full_state_lemma tr p sid init last =
-  full_state_session_lemma tr p sid (Snoc init last)
+  (ensures Some? (get_full_state p tr)
+  )
+let get_state_get_full_state tr p sid  =  
+  let (Some state, _) = get_state p sid tr in
+  get_state_state_was_set p sid tr;
+  state_was_set_full_state tr p sid state
 
 val get_state_appears_in_full_state :
   tr:trace -> p:principal -> sid:state_id ->
   Lemma
   (requires
        Some? (fst (get_state p sid tr))
-     /\ Some? (get_full_state p tr)
   )
   (ensures (
     let (Some state, _) = get_state p sid tr in
+    get_state_get_full_state tr p sid;
     let Some full_state = get_full_state p tr in
+    
     exists init. (sid, Snoc init state) `List.mem` full_state 
   )
   )
 let get_state_appears_in_full_state  tr p sid =
   let (Some state, _) = get_state p sid tr in
+
+  get_state_get_full_state tr p sid;
   let Some full_state = get_full_state p tr in
+  
   state_was_set_full_state tr p sid state;
   FStar.List.Tot.Properties.memP_map_elim fst sid full_state;
+  full_state_some_get_session_get_state p sid tr
   
-  let Some session = get_session p sid tr in
-  eliminate exists sess. (sid, sess) `List.mem` full_state
-  returns (sid, session) `List.mem` full_state
-  with _ .
-    full_state_session_lemma tr p sid sess
-  
-val get_state_get_full_state:
-  p:principal -> sid:state_id -> tr:trace ->
-  Lemma 
-    (requires True
-    )
-    (ensures (
-      let (opt_state, _) = get_state p sid tr in
-      let opt_full_state = get_full_state p tr in
-      match opt_state with
-      | None -> True
-      | Some st -> 
-          Some? opt_full_state
-    )
-    )
-let get_state_get_full_state p sid tr =
-    let (opt_state, _) = get_state p sid tr in
-      match opt_state with
-      | None -> ()
-      | Some st -> state_was_set_full_state tr p sid st
-
-
-let rec get_state_no_set_state_for_on_suffix_after_event
-  (tr:trace) (p:principal) (sid:state_id) :
-  Lemma 
-  ( let (opt_cont, tr_out) = get_state p sid tr in
-  match opt_cont with
-    | None -> True
-    | Some st -> no_set_state_entry_for p sid (tr `suffix_after_event` (SetState p sid st)) 
-  )
-  = reveal_opaque (`%get_state) get_state; 
-  match get_state p sid tr with
-  | (None, _) -> ()
-  | (Some st, _) ->
-  match tr with
-  | Nil -> ()
-  | Snoc init (SetState p' sid' cont') -> 
-         if p' = p && sid' = sid
-           then ()
-           else ( 
-             get_state_no_set_state_for_on_suffix_after_event init p sid;
-             suffix_after_event_init tr (SetState p' sid' cont')
-           )
-  | Snoc init ev -> 
-    get_state_no_set_state_for_on_suffix_after_event init p sid;
-    suffix_after_event_init tr (SetState p sid st)
-
-
-let rec no_set_state_entry_for_on_suffix (tr:trace) (suff:trace) (p:principal) (sid:state_id):
-  Lemma
-  (requires tr `has_suffix` suff /\ no_set_state_entry_for p sid tr
-  )
-  (ensures
-    no_set_state_entry_for p sid suff
-  )
-  = match suff with
-  | Nil -> ()
-  | Snoc suff_init suff_ev ->
-         match tr with
-         | Nil -> ()
-         | Snoc tr_init tr_ev -> 
-                init_is_prefix tr;
-                no_set_state_entry_for_on_suffix tr_init suff_init p sid;
-                assert(event_exists tr tr_ev)
 
