src/core/DY.Core.List.fst
@@ -1,6 +1,7 @@
 module DY.Core.List
 
 module List = FStar.List.Tot.Base
+module ListProp = FStar.List.Tot.Properties
 
 let rec choose_equals (#a #b:eqtype) (f g: a -> option b) (xs: list a):
   Lemma 
@@ -14,8 +15,6 @@ let rec choose_equals (#a #b:eqtype) (f g: a -> option b) (xs: list a):
     match xs with
     | [] -> ()
     | hd :: tl -> choose_equals f g tl
-
-
 
 let rec mem_choose (#a #b:eqtype) (f: a -> option b) (xs : list a) (x:a):
   Lemma
@@ -43,3 +42,108 @@ let rec mem_choose_elim (#a #b:eqtype) (f: a -> option b) (xs : list a) (y : b)
   | [] -> ()
   | hd :: tl -> mem_choose_elim f tl y
 
+
+let pair_elem_fst_elem (#a #b:eqtype) (p:(a * b)) (xs: list (a*b)):
+  Lemma
+  ( p `List.mem` xs ==> fst p `List.mem` (List.map fst xs)
+  )
+  [SMTPat (p `List.mem` xs) ]
+  = FStar.List.Tot.Properties.memP_map_intro fst p xs
+
+// let rec index_is_mem (#a:eqtype) (xs:list a) (i:nat{i < List.length xs}):
+//   Lemma(
+//     (xs `List.index` i) `List.mem` xs
+//   )
+//   = match xs with
+//   | [] -> ()
+//   | hd::tl ->
+//       if i = 0 
+//       then ()
+//       else index_is_mem tl ((i-1) <: nat)
+
+
+// let rec mem_has_index (#a:eqtype) (xs: list a) (x:a):
+//   Lemma
+//   (requires
+//     x `List.mem` xs
+//   )
+//   (ensures (exists i. x = List.index xs i)
+//   )
+//   = match xs with
+//   | [] -> ()
+//   | hd :: tl -> 
+//     if hd = x 
+//     then (
+//       introduce exists i. x = List.index xs i
+//       with 0
+//       and ()
+//     )
+//     else ( 
+//       mem_has_index tl x;
+//       eliminate exists i. x = List.index tl i
+//       returns (exists i. x = List.index xs i)
+//       with _ .
+//       ( introduce exists i. x = List.index xs i
+//         with (i+1) and ()
+//       )
+//     )
+
+// let distinct_mems_have_distinct_indices (#a:eqtype) (xs:list a) (x y : a):
+//   Lemma
+//   ( requires 
+//       x <> y
+//       /\ x `List.mem` xs /\ y `List.mem` xs
+//   )
+//   (ensures
+//      exists i j. x = xs `List.index` i /\ y = xs `List.index` j /\ i <> j
+//   )
+//   = mem_has_index xs x;
+//     mem_has_index xs y
+    
+
+// let rec xy (#a #b:eqtype) (f: a -> option b) (xs:list a) (y:a):
+//   Lemma
+//   (requires List.noRepeats xs
+//     /\ (forall x x'. x <> x' /\ Some? (f x) /\ Some? (f x') ==> f x <> f x')
+//     /\ Some? (f y)
+//     /\ ~ (y `List.mem` xs)
+//   )
+//   (ensures (
+//      let Some fy = f y in
+//      ~ (fy `List.mem` (List.choose f xs))
+//   )
+//   )
+// = let Some fy = f y in
+//   match xs with
+//   | [] -> ()
+//   | hd::tl -> xy f tl y
+      
+
+// let rec choose_no_repeats (#a #b:eqtype) (f: a  -> option b) (xs:list a):
+//   Lemma 
+//   ( requires 
+//       List.noRepeats xs
+//       /\ (forall x y . x <> y /\ Some? (f x) /\ Some? (f y) ==>
+//         f x <> f y)
+//   )
+//   (ensures List.noRepeats (List.choose f xs)
+//   )
+//   = match xs with
+//  | [] -> ()
+//  | hd :: tl ->
+//      match f hd with
+//      | Some x -> (
+//          choose_no_repeats f tl;
+//          xy f tl hd
+//        )
+//      | None -> choose_no_repeats f tl 
+
+
+/// The trace is a list of trace events.
+/// Because the trace grows with time and the time is often represented going from left to right,
+/// the trace is actually a reversed list.
+/// To avoid confusions, we define a custom inductive to swap the arguments of the "cons" constructor.
+
+type rev_list (a:Type) =
+  | Nil : rev_list a
+  | Snoc: rev_list a -> a -> rev_list a
