src/core/DY.Core.Trace.State.NoSetStateEntry.fst
@@ -1,0 +1,97 @@
+module DY.Core.Trace.State.NoSetStateEntry
+
+open DY.Core.Label.Type
+open DY.Core.Trace.Type
+open DY.Core.Trace.PrefixSuffix
+open DY.Core.List
+
+/// The main property we want to show is
+/// that a particular session of a principal stays the same
+/// if there are no more `SetState` entries for this principal and this session on the trace.
+
+
+
+
+/// if there are no state entries on a trace,
+/// this is true for any prefix of the trace.
+
+val no_set_state_entry_for_prefix:
+  p:principal -> sid:state_id -> tr1:trace -> tr2:trace ->
+  Lemma 
+    (requires no_set_state_entry_for p sid tr2 /\ tr1 <$ tr2)
+    (ensures no_set_state_entry_for p sid tr1)
+    [SMTPat (no_set_state_entry_for p sid tr2); SMTPat (tr1 <$ tr2)]
+let no_set_state_entry_for_prefix p sid tr1 tr2 = 
+  introduce forall (ts:timestamp{ts < length tr1}). get_event_at tr1 ts = get_event_at tr2 ts
+  with begin
+    let ev1 = get_event_at tr1 ts in
+    event_at_grows tr1 tr2 ts ev1
+    end
+
+
+/// concatenating traces without state entries
+/// results in no state entries
+#push-options "--fuel 2"
+val no_set_state_entry_for_concat:
+  p:principal -> sid:state_id ->
+  tr1: trace -> tr2:trace ->
+  Lemma
+    (requires 
+        no_set_state_entry_for p sid tr1
+      /\ no_set_state_entry_for p sid tr2
+    )
+    (ensures
+      no_set_state_entry_for p sid (tr1 `trace_concat` tr2)
+    )
+    // [SMTPat (no_set_state_entry_for p sid tr1)
+    // ; SMTPat (no_set_state_entry_for p sid tr2)]
+let rec no_set_state_entry_for_concat p sid tr1 tr2 =
+  match tr2 with
+  | Nil -> ()
+  | Snoc init2 ev2 -> 
+    init_is_prefix tr2;
+    assert(event_exists tr2 ev2);
+    no_set_state_entry_for_prefix p sid init2 tr2;
+    no_set_state_entry_for_concat p sid tr1 init2
+#pop-options
+
+/// transitivity of `no_set_state_entry_for` on suffixes of growing traces
+val no_set_state_entry_for_suffixes_transitive:
+  p:principal -> sid:state_id ->
+  tr1:trace -> tr2:trace{tr1 <$ tr2} -> tr3:trace{tr2 <$ tr3} ->
+  Lemma
+  (requires
+      no_set_state_entry_for p sid (tr2 `suffix_after` tr1)
+    /\ no_set_state_entry_for p sid (tr3 `suffix_after` tr2)
+  )
+  (ensures
+    no_set_state_entry_for p sid (tr3 `suffix_after` tr1)
+  )
+let no_set_state_entry_for_suffixes_transitive p sid tr1 tr2 tr3 =
+  suffix_after_concat tr1 tr2 tr3;
+  no_set_state_entry_for_concat p sid (tr2 `suffix_after` tr1) (tr3 `suffix_after` tr2)
+
+
+
+let no_set_state_entry_for_p (p:principal) (tr:trace) =
+  forall sid. no_set_state_entry_for p sid tr
+
+
+
+let rec no_set_state_entry_for_on_suffix (tr:trace) (suff:trace) (p:principal) (sid:state_id):
+  Lemma
+  (requires 
+    tr `has_suffix` suff /\ no_set_state_entry_for p sid tr
+  )
+  (ensures
+    no_set_state_entry_for p sid suff
+  )
+  = match suff with
+  | Nil -> ()
+  | Snoc suff_init suff_ev ->
+         match tr with
+         | Nil -> ()
+         | Snoc tr_init tr_ev -> 
+                init_is_prefix tr;
+                no_set_state_entry_for_on_suffix tr_init suff_init p sid;
+                assert(event_exists tr tr_ev)
